rt spec+proof: prove doReplyTransfer_ccorres and some other rules
This proves doReplyTransfer_ccorres, as well as the following rules
which were previously sorried or partially sorried

 - setMRs_fault_ccorres
 - handleFaultReply_ccorres
 - handleInvocation_def2

and removes cteDeleteOne_tcbFault, which is no longer necessary
for MCS.

Note that the ccorres rules for sendFaultIPC, handleTimeout, and
handleFault were moved up in Syscall_C in order to be made available
in doReplyTransfer_ccorres.

Signed-off-by: Michael McInerney <michael.mcinerney@proofcraft.systems>

proof/refine/RISCV64/TcbAcc_R.thy
@@ -2891,6 +2891,11 @@ lemma tcbSchedEnqueue_corres:
 definition weak_sch_act_wf :: "scheduler_action \<Rightarrow> kernel_state \<Rightarrow> bool" where
   "weak_sch_act_wf sa s \<equiv> \<forall>t. sa = SwitchToThread t \<longrightarrow> tcb_at' t s"
 
+defs weak_sch_act_wf_asrt_def:
+  "weak_sch_act_wf_asrt \<equiv> \<lambda>s. weak_sch_act_wf (ksSchedulerAction s) s"
+
+declare weak_sch_act_wf_asrt_def[simp]
+
 lemma weak_sch_act_wf_updates[simp]:
   "\<And>f. weak_sch_act_wf sa (ksDomainTime_update f s) = weak_sch_act_wf sa s"
   "\<And>f. weak_sch_act_wf sa (ksReprogramTimer_update f s) = weak_sch_act_wf sa s"
